backend/Constpropproof.v
@@ -20,6 +20,9 @@ Require Import Op Registers RTL.
 Require Import Liveness ValueDomain ValueAOp ValueAnalysis.
 Require Import ConstpropOp ConstpropOpproof Constprop.
 
+Section WITHROMEMFOR.
+Context `{romem_for_instance: ROMemFor}.
+
 Definition match_prog (prog tprog: program) :=
   match_program (fun cu f tf => tf = transf_fundef (romem_for cu) f) eq prog tprog.
 
@@ -29,14 +32,20 @@ Proof.
   intros. eapply match_transform_program_contextual. auto.
 Qed.
 
+End WITHROMEMFOR.
+
 Section PRESERVATION.
 Context `{external_calls_prf: ExternalCalls}.
 
 Variable prog: program.
 Variable tprog: program.
-Hypothesis TRANSL: match_prog prog tprog.
 Let ge := Genv.globalenv prog.
 Let tge := Genv.globalenv tprog.
+
+Section WITHROMEMFOR.
+Context `{romem_for_instance: ROMemFor}.
+
+Hypothesis TRANSL: match_prog prog tprog.
 
 (** * Correctness of the code transformation *)
 
@@ -593,6 +602,12 @@ Qed.
 
 End WITHWRITABLEBLOCK.
 
+End WITHROMEMFOR.
+
+Local Existing Instance romem_for_wp_instance.
+
+Hypothesis TRANSL: match_prog prog tprog.
+
 Lemma transf_initial_states:
   forall st1, initial_state prog st1 ->
   exists n, exists st2, initial_state tprog st2 /\ match_states n st1 st2.
@@ -604,6 +619,7 @@ Proof.
   apply (Genv.init_mem_match TRANSL); auto.
   replace (prog_main tprog) with (prog_main prog).
   rewrite symbols_preserved. eauto.
+  assumption.
   symmetry; eapply match_program_main; eauto.
   rewrite <- H3. apply sig_function_translated.
   constructor. auto. constructor. constructor. apply Mem.extends_refl.
@@ -640,6 +656,7 @@ Proof.
   exists n2; exists s2'; split; auto. left; apply plus_one; auto.
   exists n2; exists s2; split; auto. right; split; auto. subst t; apply star_refl.
 - apply senv_preserved.
+  assumption.
 Qed.
 
 End PRESERVATION.
