backend/Deadcodeproof.v
@@ -18,6 +18,9 @@ Require Import Values Memory Globalenvs Events Smallstep.
 Require Import Registers Op RTL.
 Require Import ValueDomain ValueAnalysis NeedDomain NeedOp Deadcode.
 
+Section WITHROMEMFOR.
+Context `{romem_for_instance: ROMemFor}.
+
 Definition match_prog (prog tprog: RTL.program) :=
   match_program (fun cu f tf => transf_fundef (romem_for cu) f = OK tf) eq prog tprog.
 
@@ -26,6 +29,8 @@ Lemma transf_program_match:
 Proof.
   intros. eapply match_transform_partial_program_contextual; eauto.
 Qed.
+
+End WITHROMEMFOR.
 
 (** * Relating the memory states *)
 
@@ -174,9 +179,13 @@ Context `{external_calls_prf: ExternalCalls}.
 
 Variable prog: program.
 Variable tprog: program.
-Hypothesis TRANSF: match_prog prog tprog.
 Let ge := Genv.globalenv prog.
 Let tge := Genv.globalenv tprog.
+
+Section WITHROMEMFOR.
+Context `{romem_for_instance: ROMemFor}.
+
+Hypothesis TRANSF: match_prog prog tprog.
 
 Lemma symbols_preserved:
   forall (s: ident), Genv.find_symbol tge s = Genv.find_symbol ge s.
@@ -908,6 +917,12 @@ Qed.
 
 End WITHWRITABLEBLOCK.
 
+End WITHROMEMFOR.
+
+Local Existing Instance romem_for_wp_instance.
+
+Hypothesis TRANSF: match_prog prog tprog.
+
 Lemma transf_initial_states:
   forall st1, initial_state prog st1 ->
   exists st2, initial_state tprog st2 /\ match_states st1 st2.
@@ -919,6 +934,7 @@ Proof.
   eapply (Genv.init_mem_match TRANSF); eauto.
   replace (prog_main tprog) with (prog_main prog). 
   rewrite symbols_preserved. eauto.
+  assumption.
   symmetry; eapply match_program_main; eauto.
   rewrite <- H3. eapply sig_function_translated; eauto.
   econstructor; eauto. constructor. apply Mem.extends_refl.
@@ -944,6 +960,7 @@ Proof.
   apply forward_simulation_step with
      (match_states := fun s1 s2 => sound_state prog s1 /\ match_states s1 s2).
 - apply senv_preserved.
+  assumption.
 - simpl; intros. exploit transf_initial_states; eauto. intros [st2 [A B]].
   exists st2; intuition. eapply sound_initial; eauto.
 - simpl; intros. destruct H. eapply transf_final_states; eauto.
